Simplification and improvements

theories/contextual_refinement.v
@@ -26,198 +26,111 @@ Section contextual_refinement.
   Context {Symbols_eq_dec: EqDecision Symbols}.
   Context {Symbols_countable: Countable Symbols}.
 
-  (** A predicate that must hold on all word of our segments
-      Typically that if it is a capability, it only points into the segment
-      (given as second argument)
+  Definition unconstrained_addr : gset Addr -> Prop :=
+    fun _ => True.
+  Lemma unconstrained_addr_union_stable:
+    ∀ dom1 dom2,
+      unconstrained_addr dom1 -> unconstrained_addr dom2 ->
+      unconstrained_addr (dom1 ∪ dom2).
+  Proof. auto. Qed.
 
-      When in doubt, instanciate this with can_address_only *)
-  Variable word_restrictions: Word -> gset Addr -> Prop.
+  Notation wf_comp := (well_formed_comp can_address_only (addr_gt_than reserved_context_size)).
+  Infix "##ₗ" := (can_link can_address_only (addr_gt_than reserved_context_size)) (at level 70).
 
-  (** Creating a link requires word_restrictions to remain true
-      as the segment increases (to the link of two segments) *)
-  Variable word_restrictions_incr:
-    forall w dom1 dom2,
-      dom1 ⊆ dom2 ->
-      word_restrictions w dom1 ->
-      word_restrictions w dom2.
-
-  (** Contextual refinement requires word_restrictions to imply
-      that capabilities only point to the given set *)
-  Variable word_restrictions_implies_address_only:
-      ∀ w dom, word_restrictions w dom -> can_address_only w dom.
-
-  (** A predicate on the addresses used by our components
-      Since memory is finite, we need have some free memory for our contexts
-      otherwise any program that takes the whole memory would refine into anything
-
-      When in doubt, instanciate this with [addr_gt_than reserved_context_size] *)
-  Variable addr_restrictions: gset Addr -> Prop.
-
-  (** Creating a link requires that addr_restriction remains true on unions *)
-  Variable addr_restrictions_union_stable:
-    forall dom1 dom2,
-      addr_restrictions dom1 ->
-      addr_restrictions dom2 ->
-      addr_restrictions (dom1 ∪ dom2).
-
-  (** Contextual refinement requires addr_restrictions to imply
-      that the first [reserved_context_size] addresses are free *)
-  Variable addr_restrictions_implies_addr_gt:
-    ∀ dom, addr_restrictions dom -> addr_gt_than reserved_context_size dom.
-
-  (** Register that holds the stack capability. Any != PC will do
-      since we quantify over all programs *)
-  Definition r_stk := r_t1.
-
-  Set Implicit Arguments.
-
-  Section definition.
-
-    (** Component with proof of their well-formedness *)
-    Record component_wf := {
-      comp : pre_component Symbols;
-      comp_is_wf : well_formed_pre_comp word_restrictions addr_restrictions comp
-    }.
-
-    (** Create a initial machine state from a component:
-        - registers are all 0, except PC which is main, and r_stk which points to the stack
-        - the memory is the one specified in the segment *)
-    Definition initial_state (c: component Symbols) :=
-      match c with
-      | Lib pre_comp => (∅, ∅) (* dummy value *)
-      | Main pre_comp c_main =>
-        (<[PC := c_main]> (gset_to_gmap (WInt 0) (list_to_set all_registers)),
-        pre_comp.(segment))
-      end.
-
-    Definition unconstrained_addr : gset Addr -> Prop :=
-      fun _ => True.
-
-    (** This is the contextual refinement relation
-        A component 'impl' contextually refines 'spec' if,
-        for all contexts 'ctxt'
-        if
-        - 'ctxt' is well formed
-        - 'ctxt' is a valid context to run 'impl'
-        - 'ctxt' linked with 'impl' terminates in a final state 'c'
-          (either HALTED or FAILED)
-        then
-        - 'ctxt' is a valid context to run 'spec'
-        - 'ctxt' linked with 'spce' also terminates in 'c' *)
-    Definition contextual_refinement impl spec :=
-      forall (context: pre_component Symbols) (main:Word) (c: ConfFlag),
-        let linked_impl := link_main_lib context impl.(comp) main in
-        let linked_spec := link_main_lib context spec.(comp) main in
-        let ctxt := Main context main in
-        well_formed_comp can_address_only unconstrained_addr ctxt ->
-        is_context can_address_only unconstrained_addr ctxt (Lib impl.(comp)) linked_impl ->
-        (exists n, machine_run n (Executable, initial_state linked_impl) = Some c) ->
-        is_context can_address_only unconstrained_addr ctxt (Lib spec.(comp)) linked_spec /\
-          (exists n, machine_run n (Executable, initial_state linked_spec) = Some c).
-  End definition.
+  (** This is the contextual refinement relation
+      A component 'impl' contextually refines 'spec' if,
+      for all contexts 'ctxt'
+      if
+      - 'ctxt' is a valid context to run 'impl' (implies that 'ctxt' is well-formed)
+      - 'ctxt' linked with 'impl' terminates in a final state 'c'
+        (either HALTED or FAILED)
+      then
+      - 'ctxt' is a valid context to run 'spec'
+      - 'ctxt' linked with 'spce' also terminates in 'c' *)
+  Inductive contextual_refinement impl spec : Prop :=
+  | ctxt_ref_intro : forall
+    (Hwf_impl : wf_comp impl)
+    (Hwf_spec : wf_comp spec)
+    (Hrefines :
+      forall (ctxt: component Symbols) (regs:Reg) (c: ConfFlag),
+        is_context can_address_only unconstrained_addr ctxt impl regs ->
+        (exists n, machine_run n (Executable, (regs, segment (link ctxt impl))) = Some c) ->
+        is_context can_address_only unconstrained_addr ctxt spec regs /\
+          exists n, machine_run n (Executable, (regs, segment (link ctxt spec))) = Some c),
+    contextual_refinement impl spec.
 
   Section facts.
-
-    (** Contextual refinement is reflexive *)
-    #[global] Instance ctxt_ref_reflexive : Reflexive contextual_refinement.
+    Lemma ctxt_ref_reflexive {comp}:
+      wf_comp comp -> contextual_refinement comp comp.
     Proof.
-      intros [impl impl_wf] context main c linked_impl linked_spec ctxt wf_context is_ctxt1 mr.
+      intros wcomp.
+      apply ctxt_ref_intro. 1,2: exact wcomp.
+      intros ctxt regs c ctxt_impl mr_ctxt_impl.
       split; assumption.
     Qed.
 
-    (** Contextual refinement is transitive *)
-    #[global] Instance ctxt_ref_transitive : Transitive contextual_refinement.
+    Instance ctxt_ref_transitive: Transitive contextual_refinement.
     Proof.
-      intros [lib_a a_wf] [lib_b b_wf] [lib_c c_wf] a_b b_c.
-      intros context main c linked_a linked_c ctxt wf_context is_ctxt_a mr_a.
-      destruct (a_b context main c wf_context is_ctxt_a mr_a) as [is_ctxt_b mr_b].
-      apply (b_c context main c wf_context is_ctxt_b mr_b).
+      intros a b c a_b b_c.
+      inversion a_b. inversion b_c.
+      apply ctxt_ref_intro; try assumption.
+      intros ctxt regs conf ctxt_a mr_ctxt_a.
+      destruct (Hrefines ctxt regs conf ctxt_a mr_ctxt_a) as [ctxt_b mr_ctxt_b].
+      apply (Hrefines0 ctxt regs conf ctxt_b mr_ctxt_b).
     Qed.
 
-    Lemma ctxt_ref_proof_irrelevance_l impl1 impl2 spec :
-      impl1.(comp) = impl2.(comp) ->
-      contextual_refinement impl1 spec ->
-      contextual_refinement impl2 spec.
+    Lemma addr_gt_than_implies_unconstrained:
+      ∀ a, addr_gt_than reserved_context_size a -> unconstrained_addr a.
+    Proof. intros. unfold unconstrained_addr. auto. Qed.
+
+    Lemma ctxt_ref_link_l {common impl spec} :
+      common ##ₗ impl -> common ##ₗ spec ->
+      contextual_refinement impl spec ->
+      contextual_refinement (link common impl) (link common spec).
     Proof.
-      intros eq1_2 impl1_spec context main c linked_impl linked_spec ctxt wf_context is_ctxt mr.
-      unfold ctxt, linked_impl in is_ctxt, mr.
-      rewrite <- eq1_2 in is_ctxt, mr.
-      apply (impl1_spec context main c wf_context is_ctxt mr).
+      intros sep_impl sep_spec impl_spec.
+      apply ctxt_ref_intro.
+      1,2: apply (link_well_formed _ can_address_only_incr _ (addr_gt_than_union_stable _));
+           assumption.
+      intros ctxt regs c ctxt_impl mr_impl.
+      inversion ctxt_impl. inversion impl_spec.
+      pose (can_link_weaken_ar addr_gt_than_implies_unconstrained sep_impl) as common_impl.
+      apply (is_context_move_in _ can_address_only_incr _ unconstrained_addr_union_stable common_impl) in ctxt_impl.
+      symmetry in Hcan_link.
+      pose (can_link_weaken_l _ _ common_impl Hcan_link) as ctxt_common.
+      pose (can_link_weaken_r _ _ common_impl Hcan_link) as ctxt_impl'.
+      symmetry in ctxt_common, ctxt_impl'.
+      rewrite (link_assoc _ can_address_only_incr _ unconstrained_addr_union_stable ctxt_common ctxt_impl' common_impl) in mr_impl.
+      destruct (Hrefines (link ctxt common) regs c ctxt_impl mr_impl) as [ctxt_spec mr_spec].
+      inversion ctxt_spec.
+      pose (can_link_weaken_ar addr_gt_than_implies_unconstrained sep_spec) as common_spec.
+      split.
+      apply (is_context_move_out _ can_address_only_incr _ unconstrained_addr_union_stable ctxt_common).
+      exact Hwr_regs. exact ctxt_spec.
+      rewrite (link_assoc _ can_address_only_incr _ unconstrained_addr_union_stable ctxt_common (can_link_weaken_l _ _ ctxt_common Hcan_link0) common_spec).
+      exact mr_spec.
     Qed.
 
-    Lemma ctxt_ref_proof_irrelevance_r impl spec1 spec2 :
-      spec1.(comp) = spec2.(comp) ->
-      contextual_refinement impl spec1 ->
-      contextual_refinement impl spec2.
+    Lemma ctxt_ref_link_r {common impl spec} :
+      common ##ₗ impl -> common ##ₗ spec ->
+      contextual_refinement impl spec ->
+      contextual_refinement (link impl common) (link spec common).
     Proof.
-      intros eq1_2 impl_spec1 context main c linked_impl linked_spec ctxt wf_context is_ctxt mr.
-      unfold contextual_refinement, linked_spec in impl_spec1.
-      rewrite eq1_2 in impl_spec1.
-      apply (impl_spec1 context main c wf_context is_ctxt mr).
+      intros common_impl common_spec impl_spec.
+      rewrite <- (link_comm _ _ common_impl).
+      rewrite <- (link_comm _ _ common_spec).
+      exact (ctxt_ref_link_l common_impl common_spec impl_spec).
     Qed.
 
-    (* Lemma ctxt_ref_of_link impl impl' impl'' spec spec' spec'' :
-      is_link word_restrictions addr_restrictions (Lib impl.(comp)) (Lib impl'.(comp)) (Lib impl''.(comp)) ->
-      is_link word_restrictions addr_restrictions (Lib spec.(comp)) (Lib spec'.(comp)) (Lib spec''.(comp)) ->
+    (* Lemma ctxt_ref_link {impl impl' spec spec'} :
+      impl ##ₗ impl' -> spec ##ₗ spec' ->
       contextual_refinement impl spec ->
       contextual_refinement impl' spec' ->
-      contextual_refinement impl'' spec''.
+      contextual_refinement (link impl impl') (link spec spec').
     Proof.
-      intros link_impl link_spec is is'.
-      intros context main c linked_impl linked_spec ctxt wf_context is_ctxt mr. *)
+      intros imp spe is is'.
+      apply (ctxt_ref_link_l imp)
+      impl *)
   End facts.
 
 End contextual_refinement.
-
-Section contextual_refinement_weaken.
-  Context `{MachineParameters}.
-
-  Context [Symbols: Type].
-  Context [Symbols_eq_dec: EqDecision Symbols].
-  Context [Symbols_countable: Countable Symbols].
-
-  Variable word_restrictions: Word -> gset Addr -> Prop.
-  Variable word_restrictions': Word -> gset Addr -> Prop.
-  Variable word_restrictions_weaken:
-    ∀ w a, word_restrictions w a -> word_restrictions' w a.
-
-  Variable addr_restrictions: gset Addr -> Prop.
-  Variable addr_restrictions': gset Addr -> Prop.
-  Variable addr_restrictions_weaken:
-    ∀ a, addr_restrictions a -> addr_restrictions' a.
-
-  Definition component_wf_weaken_word_restrictions
-    (c: @component_wf Symbols _ _ word_restrictions addr_restrictions) := {|
-    comp := c.(comp);
-    comp_is_wf := well_formed_pre_comp_weaken_word_restrictions
-      word_restrictions_weaken c.(comp_is_wf)
-  |}.
-
-  Lemma contextual_refinement_weaken_word_restrictions :
-    ∀ impl spec,
-    contextual_refinement impl spec ->
-    contextual_refinement (component_wf_weaken_word_restrictions impl) (component_wf_weaken_word_restrictions spec).
-  Proof.
-    intros impl spec impl_spec.
-    intros context main c linked_impl linked_spec ctxt wf_context is_ctxt mr.
-    apply (impl_spec context main c wf_context is_ctxt mr).
-  Qed.
-
-  Definition component_wf_weaken_addr_restrictions
-    (c: @component_wf Symbols _ _ word_restrictions addr_restrictions) := {|
-    comp := c.(comp);
-    comp_is_wf := well_formed_pre_comp_weaken_addr_restrictions
-      addr_restrictions_weaken c.(comp_is_wf)
-  |}.
-
-  Lemma contextual_refinement_weaken_addr_restrictions :
-    ∀ impl spec,
-    contextual_refinement impl spec ->
-    contextual_refinement (component_wf_weaken_addr_restrictions impl) (component_wf_weaken_addr_restrictions spec).
-  Proof.
-    intros impl spec impl_spec.
-    intros context main c linked_impl linked_spec ctxt wf_context is_ctxt mr.
-    apply (impl_spec context main c wf_context is_ctxt mr).
-  Qed.
-
-End contextual_refinement_weaken.
